src/compiler/core/Core_init.thy
@@ -284,7 +284,7 @@ definition "activate_simp_optimization = True"
 
 definition "bootstrap_floor f_x l env =
  (let (l, env) = f_x l env
-    ; l_setup = Isab_thy_ml_extended (Ml_extended (SML_compiler_env (env \<lparr> D_output_disable_thy := True
+    ; l_setup = Isab_thy_ml_extended (ML_setup (SML_compiler_env_config (env \<lparr> D_output_disable_thy := True
                                                               , D_output_header_thy := None
                                                               , D_output_position := (0, 0) \<rparr>) ))
             # l
@@ -422,7 +422,7 @@ datatype reporting = Warning
                    | Error
                    | Writeln
 
-definition "raise_ml l_out s = SML (SML.apply \<open>Ty'.check\<close>
+definition "raise_ml l_out s = SML (SML.app \<open>Ty'.check\<close>
     [ SML.list'
         (\<lambda>(rep, s).
           SML.pair (SML.basic [S.flatten [ \<open>OCL.\<close>
